Splinter/Journal/ReprJournalRefinement.i.dfy
@@ -15,8 +15,13 @@ module ReprJournalRefinement {
     var tj :=  v.journal.truncatedJournal;
     && v.WF()
     && tj.diskView.Acyclic()
-    && tj.RepresentationIsTight(v.reprIndex.Values)
-    && v.reprIndex == BuildReprIndex(tj.diskView, tj.freshestRec)
+
+    && v.reprIndex == BuildReprIndex(tj)
+
+    // todo(tony): Do we need something stronger than this? 
+    // I think we also need to say that for each lsn in key, it maps to THE UNIQUE page in the representation that contains it
+    // I think this is what we need ultimately, but we may need intermediate invariants to prove this.
+    && v.reprIndex.Values == tj.Representation()
   }
 
   lemma InvNext(v: Variables, v': Variables, lbl: TransitionLabel)
@@ -48,17 +53,67 @@ module ReprJournalRefinement {
       }
       case DiscardOldStep() => {
         // TODO
-        assume LinkedJournal.NextStep(v.journal, v'.journal, lbl, step);
-        LinkedJournalRefinement.InvNext(v.journal, v'.journal, lbl);
+        assume false;
+        // assume LinkedJournal.NextStep(v.journal, v'.journal, lbl, step);
+        // LinkedJournalRefinement.InvNext(v.journal, v'.journal, lbl);
         assert Inv(v');
       }
       case InternalJournalMarshalStep(cut) => {
         assert LinkedJournal.NextStep(v.journal, v'.journal, lbl, step);
         LinkedJournalRefinement.InvNext(v.journal, v'.journal, lbl);
+        InvNextInternalJournalMarshalStep(v, v', lbl, step);
+        BuildReprIndexGivesRepresentation(v'.journal.truncatedJournal);
         assert Inv(v');
       }
     }
   }
+
+  lemma BuildReprIndexGivesRepresentationHelper(dv: DiskView, root: Pointer) 
+    requires dv.Decodable(root)
+    requires dv.Acyclic()
+    decreases dv.TheRankOf(root)
+    ensures forall lsn | lsn in BuildReprIndexDefn(dv, root) 
+      :: lsn < dv.entries[root.value].messageSeq.seqEnd
+    ensures BuildReprIndexDefn(dv, root).Values == dv.Representation(root)
+  {
+    if root.None? {
+      assert BuildReprIndexDefn(dv, root).Values == dv.Representation(root);
+    } else {
+      BuildReprIndexGivesRepresentationHelper(dv, dv.entries[root.value].CroppedPrior(dv.boundaryLSN));
+      var currMsgs := dv.entries[root.value].messageSeq;
+      var update :=  map x: LSN | currMsgs.seqStart <= x < currMsgs.seqEnd :: root.value;
+      assert currMsgs.seqStart in update;  // witness for 0 < |update|
+    }
+  }
+
+  lemma BuildReprIndexGivesRepresentation(tj: TruncatedJournal) 
+    requires tj.WF()
+    requires tj.diskView.Decodable(tj.freshestRec)
+    requires tj.diskView.Acyclic()
+    ensures BuildReprIndex(tj).Values == tj.Representation()
+  {
+    BuildReprIndexGivesRepresentationHelper(tj.diskView, tj.freshestRec);
+  }
+
+  lemma InvNextInternalJournalMarshalStep(v: Variables, v': Variables, lbl: TransitionLabel, step: Step)
+    requires Inv(v)
+    requires v'.WF()
+    requires step.InternalJournalMarshalStep?
+    requires NextStep(v, v', lbl, step)
+    requires v'.journal.truncatedJournal.diskView.Acyclic()
+    ensures v'.reprIndex == BuildReprIndex(v'.journal.truncatedJournal)
+  {
+    var msgs := v.journal.unmarshalledTail.DiscardRecent(step.cut);
+    assert forall x | msgs.seqStart <= x < msgs.seqEnd :: x !in v.reprIndex;
+    assert lbl.addr !in v.reprIndex.Values;
+    assert v'.reprIndex.Values == v.reprIndex.Values + {lbl.addr};
+
+    // todo
+    // assert v'.journal.truncatedJournal.Representation() == v.journal.truncatedJournal.Representation() + {lbl.addr};
+    assert v'.reprIndex == BuildReprIndex(v'.journal.truncatedJournal);
+  }
+
+
 
 
 // PROVE REFINEMENT
@@ -73,135 +128,147 @@ module ReprJournalRefinement {
     ensures LinkedJournal.Init(I(v), tj)
   {}
 
-  lemma BuildTightGivesRepresentation(dv: DiskView, root: Pointer)
-    requires dv.Decodable(root)
-    requires dv.Acyclic()
-    ensures dv.BuildTight(root).entries.Keys == dv.Representation(root)
-    decreases dv.TheRankOf(root)
-  {
-    if root.Some? {
-      BuildTightGivesRepresentation(dv, dv.entries[root.value].CroppedPrior(dv.boundaryLSN));
-    }
-  }
+  // lemma BuildTightGivesRepresentation(dv: DiskView, root: Pointer)
+  //   requires dv.Decodable(root)
+  //   requires dv.Acyclic()
+  //   ensures dv.BuildTight(root).entries.Keys == dv.Representation(root)
+  //   decreases dv.TheRankOf(root)
+  // {
+  //   if root.Some? {
+  //     BuildTightGivesRepresentation(dv, dv.entries[root.value].CroppedPrior(dv.boundaryLSN));
+  //   }
+  // }
 
-  lemma BuildTightEquivalentToGarbageCollect(tj: TruncatedJournal, reprIndex: map<LSN, Address>, newBdy: LSN)
-    requires tj.WF()
-    requires tj.diskView.Acyclic()
-    requires tj.diskView.boundaryLSN <= newBdy
-    requires tj.freshestRec.Some? ==> newBdy < tj.diskView.entries[tj.freshestRec.value].messageSeq.seqEnd
-    requires reprIndex.Values == tj.diskView.Representation(tj.freshestRec);
-    requires (forall lsn :: tj.SeqStart() <= lsn < tj.SeqEnd() <==> lsn in reprIndex)
-    requires (forall lsn | lsn in reprIndex ::
-        && reprIndex[lsn] in tj.diskView.entries
-        && tj.diskView.entries[reprIndex[lsn]].ContainsLSN(lsn)
-    )
-    // requires reprIndexDiscardUpTo(reprIndex, newBdy).Values == LinkedJournal.DiskView(newBdy, MapRestrict(tj.diskView.entries, reprIndexDiscardUpTo(reprIndex, newBdy).Values)).Representation(tj.freshestRec)
-    ensures MapRestrict(tj.diskView.entries, reprIndexDiscardUpTo(reprIndex, newBdy).Values)
-      == tj.diskView.DiscardOld(newBdy).BuildTight(tj.freshestRec).entries
-  {
-    // to get the fact that DiscardOld maintains acyclicity
-    LinkedJournalRefinement.DiscardOldCommutes(tj.diskView, tj.freshestRec, newBdy);
-    assert tj.diskView.entries == tj.diskView.DiscardOld(newBdy).entries;
-    assert IsSubMap(MapRestrict(tj.diskView.entries, reprIndexDiscardUpTo(reprIndex, newBdy).Values), tj.diskView.entries);
+  // lemma LsnPageInJournal(tj: TruncatedJournal, lsn: LSN) returns (out: Address)
+  //   requires tj.WF()
+  //   requires tj.SeqStart() <= lsn < tj.SeqEnd()
+  //   ensures out in tj.diskView.entries
+  //   ensures tj.diskView.entries[out].messageSeq.seqStart <= lsn < tj.diskView.entries[out].messageSeq.seqEnd
+  //   ensures out in tj.diskView.Representation(tj.freshestRec)
+  // {
+  //   assume false;
+  // }
+
+  // lemma BuildTightEquivalentToGarbageCollect(tj: TruncatedJournal, reprIndex: map<LSN, Address>, newBdy: LSN)
+  //   requires tj.WF()
+  //   requires tj.diskView.Acyclic()
+  //   requires tj.diskView.boundaryLSN <= newBdy
+  //   requires tj.freshestRec.Some? ==> newBdy < tj.diskView.entries[tj.freshestRec.value].messageSeq.seqEnd
+  //   requires reprIndex.Values == tj.diskView.Representation(tj.freshestRec);
+  //   requires (forall lsn :: tj.SeqStart() <= lsn < tj.SeqEnd() <==> lsn in reprIndex)
+  //   requires (forall lsn | lsn in reprIndex ::
+  //       && reprIndex[lsn] in tj.diskView.entries
+  //       && tj.diskView.entries[reprIndex[lsn]].ContainsLSN(lsn)
+  //   )
+  //   ensures MapRestrict(tj.diskView.entries, reprIndexDiscardUpTo(reprIndex, newBdy).Values)
+  //     == tj.diskView.DiscardOld(newBdy).BuildTight(tj.freshestRec).entries
+  // {
+  //   // to get the fact that DiscardOld maintains acyclicity
+  //   LinkedJournalRefinement.DiscardOldCommutes(tj.diskView, tj.freshestRec, newBdy);
+  //   assert tj.diskView.entries == tj.diskView.DiscardOld(newBdy).entries;
+  //   assert IsSubMap(MapRestrict(tj.diskView.entries, reprIndexDiscardUpTo(reprIndex, newBdy).Values), tj.diskView.entries);
     
-    LinkedJournalRefinement.BuildTightIsAwesome(tj.diskView.DiscardOld(newBdy), tj.freshestRec);
-    assert IsSubMap(tj.diskView.DiscardOld(newBdy).BuildTight(tj.freshestRec).entries, tj.diskView.entries);
+  //   LinkedJournalRefinement.BuildTightIsAwesome(tj.diskView.DiscardOld(newBdy), tj.freshestRec);
+  //   assert IsSubMap(tj.diskView.DiscardOld(newBdy).BuildTight(tj.freshestRec).entries, tj.diskView.entries);
     
-    BuildTightGivesRepresentation(tj.diskView.DiscardOld(newBdy), tj.freshestRec);
-    assert tj.diskView.DiscardOld(newBdy).BuildTight(tj.freshestRec).entries.Keys == 
-      tj.diskView.DiscardOld(newBdy).Representation(tj.freshestRec);
+  //   BuildTightGivesRepresentation(tj.diskView.DiscardOld(newBdy), tj.freshestRec);
+  //   assert tj.diskView.DiscardOld(newBdy).BuildTight(tj.freshestRec).entries.Keys == 
+  //     tj.diskView.DiscardOld(newBdy).Representation(tj.freshestRec);
 
-    forall addr | addr in reprIndexDiscardUpTo(reprIndex, newBdy).Values 
-    ensures addr in tj.diskView.DiscardOld(newBdy).Representation(tj.freshestRec)
-    {
-      var newIndex := reprIndexDiscardUpTo(reprIndex, newBdy);
-      var lsn :| MapsTo(newIndex, lsn, addr);
-      
-      
+  //   forall addr | addr in reprIndexDiscardUpTo(reprIndex, newBdy).Values 
+  //   ensures addr in tj.DiscardOld(newBdy).diskView.Representation(tj.freshestRec)
+  //   {
+  //     if addr !in tj.DiscardOld(newBdy).diskView.Representation(tj.freshestRec) {
+  //       var page := tj.DiscardOld(newBdy).diskView.entries[addr];
 
-    }
+  //       // This messageSeq cannot have lsn within the operational range
+  //       assert page.messageSeq.seqEnd < newBdy || tj.SeqEnd() <= page.messageSeq.seqStart;
 
-    forall addr | addr in tj.diskView.DiscardOld(newBdy).Representation(tj.freshestRec)
-    ensures addr in reprIndexDiscardUpTo(reprIndex, newBdy).Values 
-    {
-      assume false;
-    }
+  //       assert false;
+  //     }
+  //   }
 
-    assert reprIndexDiscardUpTo(reprIndex, newBdy).Values == tj.diskView.DiscardOld(newBdy).Representation(tj.freshestRec);
-  }
+  //   forall addr | addr in tj.diskView.DiscardOld(newBdy).Representation(tj.freshestRec)
+  //   ensures addr in reprIndexDiscardUpTo(reprIndex, newBdy).Values 
+  //   {
+  //     assume false;
+  //   }
 
-  lemma DiscardOldStepRefines(v: Variables, v': Variables, lbl: TransitionLabel, step: Step)
-    requires Inv(v)
-    requires Inv(v')
-    requires NextStep(v, v', lbl, step)
-    requires step.DiscardOldStep?
-    ensures LinkedJournal.DiscardOld(I(v), I(v'), lbl)
-  {
-    var tj := v.journal.truncatedJournal;
+  //   assert reprIndexDiscardUpTo(reprIndex, newBdy).Values == tj.diskView.DiscardOld(newBdy).Representation(tj.freshestRec);
+  // }
 
-    var reprIndex' := reprIndexDiscardUpTo(v.reprIndex, lbl.startLsn);
-    var keepAddrs := reprIndex'.Values;
-    var newEntries := MapRestrict(tj.diskView.entries, keepAddrs);
-    var newDiskView := LinkedJournal.DiskView(lbl.startLsn, newEntries);
+  // lemma DiscardOldStepRefines(v: Variables, v': Variables, lbl: TransitionLabel, step: Step)
+  //   requires Inv(v)
+  //   requires Inv(v')
+  //   requires NextStep(v, v', lbl, step)
+  //   requires step.DiscardOldStep?
+  //   ensures LinkedJournal.DiscardOld(I(v), I(v'), lbl)
+  // {
+  //   var tj := v.journal.truncatedJournal;
 
-    if v.journal.truncatedJournal.SeqEnd() == lbl.startLsn {
-      assume false;
-    } else {
-      calc{
-        LinkedJournal.DiskView(lbl.startLsn, newEntries);
-        LinkedJournal.DiskView(lbl.startLsn, MapRestrict(tj.diskView.entries, keepAddrs));
-        LinkedJournal.DiskView(lbl.startLsn, MapRestrict(tj.diskView.entries, reprIndex'.Values));
-        {
-          calc {
-            MapRestrict(tj.diskView.entries, reprIndexDiscardUpTo(v.reprIndex, lbl.startLsn).Values);
-              { BuildTightEquivalentToGarbageCollect(tj, v.reprIndex, lbl.startLsn); }
-            tj.diskView.DiscardOld(lbl.startLsn).BuildTight(tj.freshestRec).entries;
-          }
-        }
-        tj.diskView.DiscardOld(lbl.startLsn).BuildTight(tj.freshestRec);
-      }
-      // calc{    
-      //   DiscardOldAndGarbageCollect(tj, lbl.startLsn, keepAddrs);
-      //   LinkedJournal.TruncatedJournal(tj.freshestRec, newDiskView);
-      //   LinkedJournal.TruncatedJournal(tj.freshestRec, LinkedJournal.DiskView(lbl.startLsn, newEntries));
-      //   // via above calc
-      //   LinkedJournal.TruncatedJournal(tj.freshestRec, tj.diskView.DiscardOld(lbl.startLsn).BuildTight(tj.freshestRec));
-      //   LinkedJournal.TruncatedJournal(tj.freshestRec, tj.diskView.DiscardOld(lbl.startLsn)).BuildTight();
-      //   tj.DiscardOld(lbl.startLsn).BuildTight();
-      // }
-    }
-    assert LinkedJournal.DiscardOld(I(v), I(v'), lbl);
-  }
+  //   var reprIndex' := reprIndexDiscardUpTo(v.reprIndex, lbl.startLsn);
+  //   var keepAddrs := reprIndex'.Values;
+  //   var newEntries := MapRestrict(tj.diskView.entries, keepAddrs);
+  //   var newDiskView := LinkedJournal.DiskView(lbl.startLsn, newEntries);
 
-  lemma NextRefines(v: Variables, v': Variables, lbl: TransitionLabel)
-    requires Inv(v)
-    requires Next(v, v', lbl)
-    ensures v'.WF()
-    ensures Inv(v')
-    ensures LinkedJournal.Next(I(v), I(v'), lbl)
-  {
-    InvNext(v, v', lbl);
-    var step: Step :| NextStep(v, v', lbl, step);
-    match step {
-      case ReadForRecoveryStep(depth) => {
-        assert LinkedJournal.NextStep(I(v), I(v'), lbl, step);
-      }
-      case FreezeForCommitStep(depth) => {
-        assert LinkedJournal.NextStep(I(v), I(v'), lbl, step);
-      } 
-      case ObserveFreshJournalStep() => {
-        assert LinkedJournal.NextStep(I(v), I(v'), lbl, step);
-      } 
-      case PutStep() => {
-        assert LinkedJournal.NextStep(I(v), I(v'), lbl, step);
-      }
-      case DiscardOldStep() => {
-        DiscardOldStepRefines(v, v', lbl, step);
-        assert LinkedJournal.NextStep(I(v), I(v'), lbl, step);
-      }
-      case InternalJournalMarshalStep(cut) => {
-        assert LinkedJournal.NextStep(I(v), I(v'), lbl, step);
-      }
-    }
-  }
+  //   if v.journal.truncatedJournal.SeqEnd() == lbl.startLsn {
+  //     assume false;
+  //   } else {
+  //     calc{
+  //       LinkedJournal.DiskView(lbl.startLsn, newEntries);
+  //       LinkedJournal.DiskView(lbl.startLsn, MapRestrict(tj.diskView.entries, keepAddrs));
+  //       LinkedJournal.DiskView(lbl.startLsn, MapRestrict(tj.diskView.entries, reprIndex'.Values));
+  //       {
+  //         calc {
+  //           MapRestrict(tj.diskView.entries, reprIndexDiscardUpTo(v.reprIndex, lbl.startLsn).Values);
+  //             { BuildTightEquivalentToGarbageCollect(tj, v.reprIndex, lbl.startLsn); }
+  //           tj.diskView.DiscardOld(lbl.startLsn).BuildTight(tj.freshestRec).entries;
+  //         }
+  //       }
+  //       tj.diskView.DiscardOld(lbl.startLsn).BuildTight(tj.freshestRec);
+  //     }
+  //     calc{    
+  //       DiscardOldAndGarbageCollect(tj, lbl.startLsn, keepAddrs);
+  //       LinkedJournal.TruncatedJournal(tj.freshestRec, newDiskView);
+  //       LinkedJournal.TruncatedJournal(tj.freshestRec, LinkedJournal.DiskView(lbl.startLsn, newEntries));
+  //       // via above calc
+  //       LinkedJournal.TruncatedJournal(tj.freshestRec, tj.diskView.DiscardOld(lbl.startLsn).BuildTight(tj.freshestRec));
+  //       LinkedJournal.TruncatedJournal(tj.freshestRec, tj.diskView.DiscardOld(lbl.startLsn)).BuildTight();
+  //       tj.DiscardOld(lbl.startLsn).BuildTight();
+  //     }
+  //   }
+  //   assert LinkedJournal.DiscardOld(I(v), I(v'), lbl);
+  // }
+
+  // lemma NextRefines(v: Variables, v': Variables, lbl: TransitionLabel)
+  //   requires Inv(v)
+  //   requires Next(v, v', lbl)
+  //   ensures v'.WF()
+  //   ensures Inv(v')
+  //   ensures LinkedJournal.Next(I(v), I(v'), lbl)
+  // {
+  //   InvNext(v, v', lbl);
+  //   var step: Step :| NextStep(v, v', lbl, step);
+  //   match step {
+  //     case ReadForRecoveryStep(depth) => {
+  //       assert LinkedJournal.NextStep(I(v), I(v'), lbl, step);
+  //     }
+  //     case FreezeForCommitStep(depth) => {
+  //       assert LinkedJournal.NextStep(I(v), I(v'), lbl, step);
+  //     } 
+  //     case ObserveFreshJournalStep() => {
+  //       assert LinkedJournal.NextStep(I(v), I(v'), lbl, step);
+  //     } 
+  //     case PutStep() => {
+  //       assert LinkedJournal.NextStep(I(v), I(v'), lbl, step);
+  //     }
+  //     case DiscardOldStep() => {
+  //       DiscardOldStepRefines(v, v', lbl, step);
+  //       assert LinkedJournal.NextStep(I(v), I(v'), lbl, step);
+  //     }
+  //     case InternalJournalMarshalStep(cut) => {
+  //       assert LinkedJournal.NextStep(I(v), I(v'), lbl, step);
+  //     }
+  //   }
+  // }
 }
